src/arch/x64/X64.Vale.StateLemmas_i.fst
@@ -6,6 +6,7 @@ module M = TransparentMap
 module BS = X64.Bytes_Semantics_s
 module ME = X64.Memory_i_s
 module TS = X64.Taint_Semantics_s
+open Taint_interop
 
 #reset-options "--initial_fuel 2 --max_fuel 2"
 
@@ -20,10 +21,10 @@ let state_to_S (s:state) : GTot TS.traceState =
   } in
   { ME.state = s'; ME.mem = s.mem});
   TS.trace = s.trace;
-  TS.memTaint = s.memTaint;
+  TS.memTaint = down_taint s.memTaint s.mem;
   }
 
-let state_of_S (s:TS.traceState) : state =
+let state_of_S (s:TS.traceState) : GTot state =
   let { ME.state = st; ME.mem = mem } = s.TS.state in
   let { BS.ok = ok; BS.regs = regs; BS.xmms = xmms; BS.flags = flags; BS.mem = _} = st in
   {
@@ -33,7 +34,7 @@ let state_of_S (s:TS.traceState) : state =
     flags = flags;
     mem = mem;
     trace = s.TS.trace;
-    memTaint = s.TS.memTaint;
+    memTaint = up_taint s.TS.memTaint mem;
   }
 
 let lemma_to_ok s = ()
@@ -42,13 +43,15 @@ let lemma_to_mem s = ()
 let lemma_to_reg s r = ()
 let lemma_to_xmm s x = ()
 let lemma_to_trace s = ()
-let lemma_to_memTaint s = ()
+let lemma_to_memTaint s = up_down_identity s.memTaint s.mem
+let lemma_to_memTaint2 s = ()
 let lemma_to_eval_operand s o = ()
 let lemma_to_eval_xmm s x = ()
 let lemma_to_valid_operand s o = ()
 let lemma_to_valid_taint s o t = ()
 
 let lemma_of_to s =
+  up_down_identity s.memTaint s.mem;
   assert (state_eq s (state_of_S (state_to_S s)));
   ()
 
@@ -62,7 +65,11 @@ let lemma_to_of s =
   assert (feq regs regs'');
   assert (feq xmms xmms'');
   ME.same_heap s.TS.state s''.TS.state;
+  down_up_identity s.TS.memTaint mem;
   ()
+
+let lemma_valid_taint64 b memTaint mem i t = admit()
+let lemma_valid_taint128 b memTaint mem i t = admit()
 
 let modify_trace s0 b =
   let s1 = {s0 with trace = BranchPredicate(b)::s0.trace} in
@@ -70,3 +77,6 @@ let modify_trace s0 b =
   let s1' = state_to_S s1 in
   assert (FunctionalExtensionality.feq s0'.TS.state.ME.state.BS.regs s1'.TS.state.ME.state.BS.regs);
   assert (FunctionalExtensionality.feq s0'.TS.state.ME.state.BS.xmms s1'.TS.state.ME.state.BS.xmms)  
+
+let same_memTaint b mem0 mem1 memtaint0 memtaint1 = admit()
+let same_memTaint128 b mem0 mem1 memtaint0 memtaint1 = admit()
