src/arch/x64/X64.Vale.Decls_i.fsti
@@ -77,8 +77,6 @@ unfold let modifies_mem (s:M.loc) (h1 h2:M.mem) : GTot Type0 = M.modifies s h1 h
 unfold let loc_buffer(#t:M.typ) (b:M.buffer t) = M.loc_buffer #t b
 unfold let locs_disjoint = M.locs_disjoint
 unfold let loc_union = M.loc_union
-unfold let modifies_memTaint (a:int) (m1 m2: map int taint) : GTot Type0 =
-m2 == Map.upd m1 a Public \/ m2 == Map.upd m1 a Secret
 
 
 (* Constructors *)
@@ -157,7 +155,7 @@ let va_opr_lemma_Mem (s:va_state) (base:operand) (offset:int) (b:M.buffer64) (in
 [@va_qattr] unfold let va_get_xmm (x:xmm) (s:va_state) : quad32 = eval_xmm x s
 [@va_qattr] unfold let va_get_mem (s:va_state) : M.mem = s.mem
 [@va_qattr] unfold let va_get_trace (s:va_state) : list observation = s.trace
-[@va_qattr] unfold let va_get_memTaint (s:va_state) : map int taint = s.memTaint
+[@va_qattr] unfold let va_get_memTaint (s:va_state) : Memtaint_i.t = s.memTaint
 
 [@va_qattr] let va_upd_ok (ok:bool) (s:state) : state = { s with ok = ok }
 [@va_qattr] let va_upd_flags (flags:nat64) (s:state) : state = { s with flags = flags }
@@ -165,7 +163,6 @@ let va_opr_lemma_Mem (s:va_state) (base:operand) (offset:int) (b:M.buffer64) (in
 [@va_qattr] let va_upd_reg (r:reg) (v:nat64) (s:state) : state = update_reg r v s
 [@va_qattr] let va_upd_xmm (x:xmm) (v:quad32) (s:state) : state = update_xmm x v s
 [@va_qattr] let va_upd_trace (trace:list observation) (s:state) : state = { s with trace=trace }
-[@va_qattr] let va_upd_memTaint (memTaint:map int taint) (s:state) : state = { s with memTaint = memTaint }
 
 (* Framing: va_update_foo means the two states are the same except for foo *)
 [@va_qattr] unfold let va_update_ok (sM:va_state) (sK:va_state) : va_state = va_upd_ok sM.ok sK
@@ -176,7 +173,6 @@ let va_opr_lemma_Mem (s:va_state) (base:operand) (offset:int) (b:M.buffer64) (in
 [@va_qattr] unfold let va_update_xmm (x:xmm) (sM:va_state) (sK:va_state) : va_state =
   va_upd_xmm x (eval_xmm x sM) sK
 [@va_qattr] unfold let va_update_trace (sM:va_state) (sK:va_state) : va_state = va_upd_trace sM.trace sK
-[@va_qattr] unfold let va_update_memTaint (sM:va_state) (sK:va_state) : va_state = va_upd_memTaint sM.memTaint sK
 
 [@va_qattr]
 let va_update_operand (o:operand) (sM:va_state) (sK:va_state) : va_state =
@@ -297,25 +293,27 @@ unfold let modifies_buffer_2 (b1 b2:M.buffer64) (h1 h2:M.mem) =modifies_mem (M.l
 unfold let modifies_buffer128 (b:M.buffer128) (h1 h2:M.mem) = modifies_mem (loc_buffer b) h1 h2
 unfold let modifies_buffer128_2 (b1 b2:M.buffer128) (h1 h2:M.mem) = modifies_mem (M.loc_union (loc_buffer b1) (loc_buffer b2)) h1 h2
 
-let validSrcAddrs64 (m:M.mem) (addr:int) (b:M.buffer64) (len:int) (memTaint:map int taint) (t:taint) =
+let validSrcAddrs64 (m:M.mem) (addr:int) (b:M.buffer64) (len:int) (memTaint:Memtaint_i.t) (t:taint) =
     buffer_readable m b /\
     len <= buffer_length b /\
     M.buffer_addr b m == addr /\ 
-    (forall a. 0 <= a && a <= len ==>
-      memTaint.[addr + 8 `op_Multiply` a] == t)
+    memTaint (Memtaint_i.Buffer (M.TBase M.TUInt64) b) == t
 
 unfold 
 let validDstAddrs64 = validSrcAddrs64
 
-let validSrcAddrs128 (m:M.mem) (addr:int) (b:M.buffer128) (len:int) =
+let validSrcAddrs128 (m:M.mem) (addr:int) (b:M.buffer128) (len:int) (memTaint:Memtaint_i.t) (t:taint) =
     buffer_readable m b /\
     len <= buffer_length b /\
-    M.buffer_addr b m == addr
+    M.buffer_addr b m == addr /\
+    memTaint (Memtaint_i.Buffer (M.TBase M.TUInt128) b) == t
 
-let validDstAddrs128 (m:M.mem) (addr:int) (b:M.buffer128) (len:int) =
+let validDstAddrs128 (m:M.mem) (addr:int) (b:M.buffer128) (len:int) (memTaint:Memtaint_i.t) (t:taint) =
     buffer_readable m b /\
     len <= buffer_length b /\
-    M.buffer_addr b m == addr
+    M.buffer_addr b m == addr /\
+    memTaint (Memtaint_i.Buffer (M.TBase M.TUInt128) b) == t
+
 
 let valid_stack_slots (m:M.mem) (rsp:int) (b:M.buffer64) (num_slots:int) =
     buffer_readable m b /\
@@ -403,38 +401,32 @@ val lemma_cmp_gt : s:va_state -> o1:va_operand -> o2:va_operand -> Lemma
 
 val lemma_valid_cmp_eq : s:va_state -> o1:va_operand -> o2:va_operand -> Lemma
   (requires True)
-  (ensures  (valid_operand o1 s /\ valid_operand o2 s 
-  /\ valid_taint o1 s Public /\ valid_taint o2 s Public) ==> (valid_ocmp (va_cmp_eq o1 o2) s))
+  (ensures  (valid_operand o1 s /\ valid_operand o2 s) ==> (valid_ocmp (va_cmp_eq o1 o2) s))
   [SMTPat (valid_ocmp (va_cmp_eq o1 o2) s)]
 
 val lemma_valid_cmp_ne : s:va_state -> o1:va_operand -> o2:va_operand -> Lemma
   (requires True)
-  (ensures (valid_operand o1 s /\ valid_operand o2 s
-   /\ valid_taint o1 s Public /\ valid_taint o2 s Public) ==> (valid_ocmp (va_cmp_ne o1 o2) s))
+  (ensures (valid_operand o1 s /\ valid_operand o2 s) ==> (valid_ocmp (va_cmp_ne o1 o2) s))
   [SMTPat (valid_ocmp (va_cmp_ne o1 o2) s)]
 
 val lemma_valid_cmp_le : s:va_state -> o1:va_operand -> o2:va_operand -> Lemma
   (requires True)
-  (ensures (valid_operand o1 s /\ valid_operand o2 s
-   /\ valid_taint o1 s Public /\ valid_taint o2 s Public) ==> (valid_ocmp (va_cmp_le o1 o2) s))
+  (ensures (valid_operand o1 s /\ valid_operand o2 s) ==> (valid_ocmp (va_cmp_le o1 o2) s))
   [SMTPat (valid_ocmp (va_cmp_le o1 o2) s)]
 
 val lemma_valid_cmp_ge : s:va_state -> o1:va_operand -> o2:va_operand -> Lemma
   (requires True)
-  (ensures (valid_operand o1 s /\ valid_operand o2 s
-   /\ valid_taint o1 s Public /\ valid_taint o2 s Public) ==> (valid_ocmp (va_cmp_ge o1 o2) s))
+  (ensures (valid_operand o1 s /\ valid_operand o2 s) ==> (valid_ocmp (va_cmp_ge o1 o2) s))
   [SMTPat (valid_ocmp (va_cmp_ge o1 o2) s)]
 
 val lemma_valid_cmp_lt : s:va_state -> o1:va_operand -> o2:va_operand -> Lemma
   (requires True)
-  (ensures (valid_operand o1 s /\ valid_operand o2 s
-   /\ valid_taint o1 s Public /\ valid_taint o2 s Public) ==> (valid_ocmp (va_cmp_lt o1 o2) s))
+  (ensures (valid_operand o1 s /\ valid_operand o2 s) ==> (valid_ocmp (va_cmp_lt o1 o2) s))
   [SMTPat (valid_ocmp (va_cmp_lt o1 o2) s)]
 
 val lemma_valid_cmp_gt : s:va_state -> o1:va_operand -> o2:va_operand -> Lemma
   (requires True)
-  (ensures (valid_operand o1 s /\ valid_operand o2 s
-   /\ valid_taint o1 s Public /\ valid_taint o2 s Public) ==> (valid_ocmp (va_cmp_gt o1 o2) s))
+  (ensures (valid_operand o1 s /\ valid_operand o2 s) ==> (valid_ocmp (va_cmp_gt o1 o2) s))
   [SMTPat (valid_ocmp (va_cmp_gt o1 o2) s)]
 
 val va_compute_merge_total (f0:va_fuel) (fM:va_fuel) : va_fuel
