src/arch/x64/X64.Vale.StateLemmas_i.fsti
@@ -7,6 +7,8 @@ module M = TransparentMap
 module BS = X64.Bytes_Semantics_s
 module ME = X64.Memory_i_s
 module TS = X64.Taint_Semantics_s
+module MT = X64.Vale.Memtaint_i
+open Taint_interop
 
 unfold let ok' s = s.ME.state.BS.ok
 unfold let regs' s = s.ME.state.BS.regs
@@ -17,7 +19,7 @@ unfold let trace' = TS.MktraceState?.trace
 unfold let memTaint' = TS.MktraceState?.memTaint
 
 val state_to_S : s:state -> GTot TS.traceState
-val state_of_S : s:TS.traceState -> state
+val state_of_S : s:TS.traceState -> GTot state
 
 val lemma_to_ok : s:state -> Lemma
   (ensures s.ok == ok' (state_to_S s).TS.state)
@@ -45,7 +47,11 @@ val lemma_to_trace : s:state -> Lemma
   [SMTPat s.trace]
 
 val lemma_to_memTaint : s:state -> Lemma
-  (ensures s.memTaint == memTaint' (state_to_S s))
+  (ensures s.memTaint == up_taint (memTaint' (state_to_S s)) s.mem)
+  [SMTPat s.memTaint]
+
+val lemma_to_memTaint2 : s:state -> Lemma
+  (ensures down_taint s.memTaint s.mem == memTaint' (state_to_S s))
   [SMTPat s.memTaint]
 
 val lemma_to_eval_operand : s:state -> o:operand -> Lemma
@@ -60,10 +66,6 @@ val lemma_to_valid_operand : s:state -> o:operand -> Lemma
   (ensures valid_operand o s ==> S.valid_operand o (state_to_S s).TS.state)
   [SMTPat (valid_operand o s)]
 
-val lemma_to_valid_taint : s:state -> o:operand -> t:taint -> Lemma
-  (ensures valid_taint o s t ==> TS.taint_match o t (state_to_S s).TS.memTaint (state_to_S s).TS.state)
-  [SMTPat (valid_taint o s t)]
-
 val lemma_of_to : s:state -> Lemma
   (ensures s == state_of_S (state_to_S s))
   [SMTPat (state_of_S (state_to_S s))]
@@ -72,5 +74,40 @@ val lemma_to_of : s:TS.traceState -> Lemma
   (ensures s == state_to_S (state_of_S s))
   [SMTPat (state_to_S (state_of_S s))]
 
+val lemma_valid_taint64: (b:X64.Memory_i.buffer64) ->
+			 (memTaint:MT.t) ->
+			 (mem:X64.Memory_i.mem) ->
+			 (i:nat{i < X64.Memory_i.buffer_length b}) ->
+			 (t:taint) -> Lemma
+  (requires valid_taint_buf64 b memTaint t)
+  (ensures (down_taint memTaint mem).[X64.Memory_i.buffer_addr b mem + 8 `op_Multiply` i] == t)
+
+val lemma_valid_taint128: (b:X64.Memory_i.buffer128) ->
+			 (memTaint:MT.t) ->
+			 (mem:X64.Memory_i.mem) ->
+			 (i:nat{i < X64.Memory_i.buffer_length b}) ->
+			 (t:taint) -> Lemma
+  (requires valid_taint_buf128 b memTaint t)
+  (ensures (down_taint memTaint mem).[X64.Memory_i.buffer_addr b mem + 16 `op_Multiply` i] == t)
+
+
 val modify_trace: (s0:state) -> (b:bool) -> Lemma
   (state_to_S ({s0 with trace=BranchPredicate(b)::s0.trace}) == ({(state_to_S s0) with TS.trace = BranchPredicate(b)::(state_to_S s0).TS.trace}))
+
+val same_memTaint: (b:X64.Memory_i.buffer64) -> 
+                   (mem0:X64.Memory_i.mem) ->
+		   (mem1:X64.Memory_i.mem) ->
+		   (memtaint0:MT.t) ->
+		   (memtaint1:MT.t) -> Lemma
+  (requires (X64.Memory_i.modifies (X64.Memory_i.loc_buffer b) mem0 mem1 /\ 
+    (forall p. Map.sel (down_taint memtaint0 mem0) p == Map.sel (down_taint memtaint1 mem1) p)))
+  (ensures memtaint0 == memtaint1)
+
+val same_memTaint128: (b:X64.Memory_i.buffer128) -> 
+                   (mem0:X64.Memory_i.mem) ->
+		   (mem1:X64.Memory_i.mem) ->
+		   (memtaint0:MT.t) ->
+		   (memtaint1:MT.t) -> Lemma
+  (requires (X64.Memory_i.modifies (X64.Memory_i.loc_buffer b) mem0 mem1 /\ 
+    (forall p. Map.sel (down_taint memtaint0 mem0) p == Map.sel (down_taint memtaint1 mem1) p)))
+  (ensures memtaint0 == memtaint1)
