src/crypto/poly1305/x64/X64.Poly1305.Util_i.fsti
@@ -73,12 +73,11 @@ match l with
 
 unfold let modifies_buffer (b:buffer64) (h1 h2:mem) = modifies_mem (loc_buffer b) h1 h2
 
-let validSrcAddrs64 (m:mem) (addr:int) (b:buffer64) (len:int) (memTaint:map int taint) (t:taint) =
+let validSrcAddrs64 (m:mem) (addr:int) (b:buffer64) (len:int) (memTaint:X64.Vale.Memtaint_i.t) (t:taint) =
     buffer_readable m b /\
     len <= buffer_length b /\
     buffer_addr b m == addr /\
-    (forall a. 0 <= a && a <= len ==>
-      memTaint.[addr + 8 `op_Multiply` a] == t)    
+    valid_taint_buf64 b memTaint t
 
 let modifies_buffer_specific (b:buffer64) (h1 h2:mem) (start last:nat) : GTot Type0 =
     modifies_buffer b h1 h2 /\
@@ -94,8 +93,3 @@ unfold let buffers_disjoint (b1 b2:buffer64) =
 
 let readable_words (len:nat) =
     ((len + 15) / 16) `op_Multiply` 2 // 2 == 16 for rounding /8 for 8-byte words
-
-let apply_valid_taint (i:int) (r_value:nat) (mem:mem) (t:taint) (length:int) (memTaint:map int taint) (ctx_b:buffer64) (inp_b:buffer64) : Lemma
-    (requires length >= 0 /\ validSrcAddrs64 mem r_value inp_b (length `op_Division` 8) memTaint t /\ 0 <= i /\ i <= length `op_Division` 8)
-    (ensures length >= 0 /\ valid_taint_ptr (r_value + 8 `op_Multiply` i) memTaint t) =
-  ()
